Added compileDefine, which deals with some ARM peculiarities, such as small immediate constants, and also tries to get functions into the particular form needed by Magnus' backend.

examples/dev/sw2/test/tea.sml
@@ -19,6 +19,12 @@ val KMATCH_MP_TAC =
   Ho_Rewrite.REWRITE_RULE [AND_IMP_INTRO,
            METIS_PROVE [] ``(a ==> !x. b x) = !x. a ==> b x``]; 
 
+val WORD_PRED_EXISTS = Q.prove
+(`!w:'a word. ~(w = 0w) ==> ?u. w = u + 1w`,
+  RW_TAC std_ss [] THEN 
+  Q.EXISTS_TAC `w - 1w` THEN 
+  RW_TAC std_ss [WORD_SUB_ADD,WORD_ADD_SUB,WORD_MULT_CLAUSES]);
+
 
 (*---------------------------------------------------------------------------*)
 (* Cipher types                                                              *)
@@ -57,6 +63,7 @@ val Rounds_def =
    `Rounds (n:word32,s:state) = 
       if n=0w then s else Rounds (n-1w, Round s)`;
 
+val Rounds_ind = fetch "-" "Rounds_ind";
 
 (*---------------------------------------------------------------------------*)
 (* Encrypt  (32 rounds)                                                      *)
@@ -101,49 +108,44 @@ val InvRounds_def =
 val TEADecrypt_def =
  Define
    `TEADecrypt (keys,txt) =
-      let (plaintxt,keys,sum) = InvRounds(32w,(txt,keys,DELTA << 5)) in
-      plaintxt`;
+      let (plaintxt,keys,sum) = InvRounds(32w,(txt,keys,DELTA << 5)) 
+      in
+        plaintxt`;
 
 (*===========================================================================*)
 (* Correctness                                                               *)
 (*===========================================================================*)
 
 (*---------------------------------------------------------------------------*)
-(* Case analysis on a block and a key and a state		             *)
+(* Case analysis on a state                                                  *)
 (*---------------------------------------------------------------------------*)
-
-val WORD_PRED_EXISTS = Q.prove
-(`!w:'a word. ~(w = 0w) ==> ?u. w = u + 1w`,
-  RW_TAC std_ss [] THEN 
-  Q.EXISTS_TAC `w - 1w` THEN 
-  RW_TAC std_ss [WORD_SUB_ADD,WORD_ADD_SUB,WORD_MULT_CLAUSES]);
 
 val FORALL_STATE = Q.prove
  (`(!x:state. P x) = !v0 v1 k0 k1 k2 k3 sum. P((v0,v1),(k0,k1,k2,k3),sum)`,
     METIS_TAC [PAIR]
  );
 
+(*---------------------------------------------------------------------------*)
+(* Basic inversion lemma                                                     *)
+(*---------------------------------------------------------------------------*)
+
 val OneRound_Inversion = Q.store_thm("OneRound_Inversion",
  `!s:state. InvRound (Round s) = s`,
  SIMP_TAC std_ss [FORALL_STATE] THEN
  RW_TAC list_ss [Round_def, InvRound_def,WORD_ADD_SUB, LET_THM]);
 
-
-val Rounds_ind = fetch "-" "Rounds_ind";
-
-val th = 
- GEN_ALL(SIMP_RULE std_ss [FORALL_PROD]
-   (GEN_BETA_RULE
-    (Q.ISPEC `\(a:word32,b:state). P (a,FST(b), FST(SND(b)), SND(SND b)):bool` 
-     Rounds_ind)));
+(*---------------------------------------------------------------------------*)
+(* Specialized version of Rounds induction.                                  *)
+(*---------------------------------------------------------------------------*)
 
 val Rounds_ind' = Q.prove
 (`!P. 
    (!(n:word32) b1 k1 s1. 
        (~(n = 0w) ==> P (n - 1w,Round(b1,k1,s1))) ==> P (n,(b1,k1,s1))) ==>
      !i b k s:word32. P (i,b,k,s)`,
- SIMP_TAC std_ss [FORALL_PROD] THEN GEN_TAC THEN DISCH_TAC THEN 
- HO_MATCH_MP_TAC th THEN RW_TAC std_ss []);
+ REPEAT STRIP_TAC THEN 
+ MATCH_MP_TAC (DISCH_ALL(SPEC_ALL (UNDISCH (SPEC_ALL Rounds_ind)))) THEN
+ METIS_TAC [ABS_PAIR_THM]);
 
 (*---------------------------------------------------------------------------*)
 (* Main lemmas                                                               *)
@@ -169,9 +171,6 @@ val delta_shift = Q.prove
 (`DELTA << 5 = DELTA * 32w`, 
  REWRITE_TAC [DELTA_def] THEN WORDS_TAC);
 
-val [Round,InvRound,DELTA] = flatten(map decls ["Round", "InvRound", "DELTA"]);
-val RESTR_EVAL_TAC = computeLib.RESTR_EVAL_TAC;
-
 (*---------------------------------------------------------------------------*)
 (* Basic theorem about encryption/decryption                                 *)
 (*---------------------------------------------------------------------------*)
@@ -180,13 +179,15 @@ val TEA_CORRECT = Q.store_thm
 ("TEA_CORRECT",
  `!plaintext keys.
      TEADecrypt (keys,TEAEncrypt (keys,plaintext)) = plaintext`,
-   RW_TAC list_ss [TEAEncrypt_def, TEADecrypt_def,delta_shift] THEN
-   `(keys1=keys) /\ (sum = DELTA*32w)` 
-     by METIS_TAC[lemma2,WORD_ADD_0,PAIR_EQ]THEN RW_TAC std_ss [] THEN
-   Q.PAT_ASSUM `Rounds x = y` (SUBST_ALL_TAC o SYM) THEN
-   POP_ASSUM MP_TAC THEN RESTR_EVAL_TAC [Round, InvRound, DELTA] THEN 
-   RW_TAC std_ss [OneRound_Inversion]
- );
+ RW_TAC list_ss [TEAEncrypt_def, TEADecrypt_def, delta_shift] 
+  THEN `(keys1 = keys) /\ (sum = DELTA * 32w)` 
+        by METIS_TAC [lemma2,WORD_ADD_0,PAIR_EQ] 
+  THEN RW_TAC std_ss [] 
+  THEN Q.PAT_ASSUM `Rounds x = y` (SUBST_ALL_TAC o SYM) 
+  THEN POP_ASSUM MP_TAC 
+  THEN computeLib.RESTR_EVAL_TAC 
+           (flatten(map decls ["Round", "InvRound", "DELTA"])) 
+  THEN RW_TAC std_ss [OneRound_Inversion]);
 
 
 (*===========================================================================*)
